mppa_k1c/Asmblockgenproof.v
@@ -523,7 +523,7 @@ Proof.
   - simpl in TIB. unfold transl_load in TIB. exploreInst; try discriminate.
     all: monadInv TIB; unfold transl_memory_access in EQ0; unfold transl_memory_access2 in EQ0; unfold transl_memory_access2XS in EQ0; exploreInst; try discriminate.
   - simpl in TIB. unfold transl_store in TIB. exploreInst; try discriminate.
-    all: monadInv TIB; unfold transl_memory_access in EQ0; unfold transl_memory_access2 in EQ0; exploreInst; try discriminate.
+    all: monadInv TIB; unfold transl_memory_access in EQ0; unfold transl_memory_access2 in EQ0; unfold transl_memory_access2XS in EQ0; exploreInst; try discriminate. 
 Qed.
 
 Lemma transl_basic_code_nonil:
